fitree: basic definitions for finite ITrees (fitree)

MLIRSemantics.lean
@@ -1,1 +1,78 @@
-def hello := "world"
+/- Extendable effect families -/
+
+def to1 (E F: Type → Type) :=
+  ∀ T, E T → F T
+def sum1 (E F: Type → Type) :=
+  fun T => E T ⊕ F T
+inductive void1: Type -> Type
+
+infixr:40 " ~> " => to1
+
+class Member (E F: Type → Type) where
+  inject : E ~> F
+
+instance {E}: Member E E where
+  inject := (fun _ => id)
+
+instance {E F G} [Member E F]: Member E (sum1 F G) where
+  inject T := Sum.inl ∘ Member.inject T
+
+instance {E F G} [Member E G]: Member E (sum1 F G) where
+  inject T := Sum.inr ∘ Member.inject T
+
+-- Effects can now be put in context automatically by typeclass resolution
+example (E: Type → Type): Member E E := inferInstance
+example (E F: Type → Type): Member E (sum1 E F) := inferInstance
+example (E F: Type → Type): Member E (sum1 F (sum1 F E)) := inferInstance
+
+
+/- Examples of interactions -/
+
+inductive stateE {S: Type}: Type → Type where
+  | Read: Unit → stateE S
+  | Write: S → stateE Unit
+
+inductive writeE {W: Type}: Type → Type where
+  | Tell: W → writeE Unit
+
+
+/- The monadic domain; essentially finite Interaction Trees -/
+
+inductive fitree (E: Type → Type) (R: Type) where
+  | Ret (r: R): fitree E R
+  | Vis {T: Type} (e: E T) (k: T → fitree E R): fitree E R
+
+def fitree.ret {E R}: R → fitree E R :=
+  fitree.Ret
+
+def fitree.trigger {E F: Type → Type} {T} [Member E F] (e: E T): fitree F T :=
+  fitree.Vis (Member.inject _ e) fitree.ret
+
+def fitree.bind {E R T} (t: fitree E T) (k: T → fitree E R) :=
+  match t with
+  | Ret r => k r
+  | Vis e k' => Vis e (λ r => bind (k' r) k)
+
+instance {E}: Monad (fitree E) where
+  pure := fitree.ret
+  bind := fitree.bind
+
+
+-- Interpretation into the monad of finite ITrees
+def interp {M} [Monad M] {E} (h: forall ⦃T⦄, E T → M T):
+    forall ⦃R⦄, fitree E R → M R :=
+  λ _ t =>
+    match t with
+    | fitree.Ret r => pure r
+    | fitree.Vis e k => bind (h e) (λ t => interp h (k t))
+
+-- Interpretation into the state monad
+def interp_state {M S} [Monad M] {E} (h: forall ⦃T⦄, E T → StateT S M T):
+    forall ⦃R⦄, fitree E R → StateT S M R :=
+  interp h
+
+-- Since we only use finite ITrees, we can actually run them when they're
+-- fully interpreted (which leaves only the Ret constructor)
+def fitree.run {R}: fitree void1 R → R
+  | Ret r => r
+  | Vis e k => nomatch e
